coq/splitting/named_prop.v
@@ -362,7 +362,6 @@ Fixpoint envs_delete_list {PROP}
     envs_delete true ih cb Δ'
   end.
 
-
 Definition envs_split {PROP}
   (bs : list bool) (Δ : envs PROP) : option (envs PROP * envs PROP) :=
   ''(Δ1,Δ2) ← env_split_go bs (env_spatial Δ);
@@ -757,53 +756,3 @@ Proof.
   apply (env_split_go_sound _ _ bs). done.
 Qed.
 End envs.
-
-Notation "" := Enil (only printing) : proof_scope.
-Notation "Γ H : P" := (Esnoc Γ (INamed H) P%I)
-  (at level 1, P at level 200,
-   left associativity, format "Γ H  :  '[' P ']' '//'", only printing) : proof_scope.
-Notation "Γ '_' : P" := (Esnoc Γ (IAnon _) P%I)
-  (at level 1, P at level 200,
-   left associativity, format "Γ '_'  :  '[' P ']' '//'", only printing) : proof_scope.
-
-Set Default Proof Using "Type".
-Delimit Scope proof_scope with env.
-Arguments Envs _ _%proof_scope _%proof_scope _.
-Arguments Enil {_}.
-Arguments Esnoc {_} _%proof_scope _%string _%I.
-
-Notation "" := Enil (only printing) : proof_scope.
-
-Notation "Γ '⟨?⟩' H : P" := (Esnoc Γ (_, INamed H) P%I)
-  (at level 1, P at level 200,
-   left associativity, format "Γ  '⟨?⟩' H  :  '[' P ']' '//'", only printing) : proof_scope.
-Notation "Γ '⟨?⟩_' : P" := (Esnoc Γ (_, IAnon _) P%I)
-  (at level 1, P at level 200,
-   left associativity, format "Γ  '⟨?⟩_'  :  '[' P ']' '//'", only printing) : proof_scope.
-
-Notation "Γ H : P" := (Esnoc Γ (true, INamed H) P%I)
-  (at level 1, P at level 200,
-   left associativity, format "Γ  H  :  '[' P ']' '//'", only printing) : proof_scope.
-Notation "Γ '_' : P" := (Esnoc Γ (true, IAnon _) P%I)
-  (at level 1, P at level 200,
-   left associativity, format "Γ  '_'  :  '[' P ']' '//'", only printing) : proof_scope.
-
-Notation "Γ" := (Esnoc Γ (false, _) _%I)
-  (at level 1, left associativity, format "Γ '//'", only printing) : proof_scope.
-
-
-Notation "Γ '--------------------------------------' □ Δ '--------------------------------------' ∗ Q" :=
-  (envs_entails (Envs Γ Δ _) Q%I)
-  (at level 1, Q at level 200, left associativity,
-  format "Γ '--------------------------------------' □ '//' Δ '--------------------------------------' ∗ '//' Q '//'", only printing) :
-  stdpp_scope.
-Notation "Δ '--------------------------------------' ∗ Q" :=
-  (envs_entails (Envs Enil Δ _) Q%I)
-  (at level 1, Q at level 200, left associativity,
-  format "Δ '--------------------------------------' ∗ '//' Q '//'", only printing) : stdpp_scope.
-Notation "Γ '--------------------------------------' □ Q" :=
-  (envs_entails (Envs Γ Enil _) Q%I)
-  (at level 1, Q at level 200, left associativity,
-  format "Γ '--------------------------------------' □ '//' Q '//'", only printing)  : stdpp_scope.
-Notation "'--------------------------------------' ∗ Q" := (envs_entails (Envs Enil Enil _) Q%I)
-  (at level 1, Q at level 200, format "'--------------------------------------' ∗ '//' Q '//'", only printing) : stdpp_scope.
