coq/splitting/tactics.v
@@ -1,0 +1,3 @@
+From Local Require Export splitting_ltac2_tactics.
+
+From iris.proofmode Require Import class_instances_bi class_instances_sbi frame_instances modality_instances.
