coq/splitting/test_imatch.v
@@ -8,18 +8,19 @@ Implicit Types P Q R : PROP.
 From Local Require Import splitting_imatch splitting_ltac2_tactics named_prop.
 Set Ltac2 Backtrace.
 
-Lemma test1 P Q : Q ⊢ □ (<absorb> P) -∗ Q.
+Lemma test1 P Q : Q ⊢ □ (<absorb> P) -∗ (* P ∗*) Q.
 Proof.
   i_start_split_proof ().
   i_intro_ident '(INamed "q").
   (* i_intro_ident '(INamed "p"). *)
   i_intro_intuitionistic_ident '(INamed "p").
+  (* i_split ().*)
   iLazyMatch! goal with
   | [h1 : <?> ?p |- _] => Message.print (oc p)
   end.
 
   iMatch! goal with
   | [h1 : _, h2 : (<absorb> _)%I |- ?p] =>
-    i_exact h1
+    i_assumption ()
   end.
 Qed.
